Field ops with map.of_list_word_at precondition
Using map.of_list_word_at instead of FElem/Bignum/array will make it a
bit easier to handle allocation of bigger chunks of memory that are then
partially fed into field operations to fill them with values.

map.of_list_word_at requires a lenght assumption, which is wrapped into
Placeholder.

The main difference between of_list_word_at and FElem is that one allows
for equational reasoning (below Placeholder) while the other one does
not need an explicit length assumption, as separation logic has it
inherently.

As far as I understand it, both FElem and Placeholder have
their advantages and disadvantages, this change hopefull allows to
switch a bit more freely between them.

I've also removed some duplicated list byte <-> list word translations
and removed unnecessary imports when I saw them.

src/Bedrock/End2End/X25519/EdwardsXYZT.v
@@ -1,4 +1,5 @@
 Require Import bedrock2.Array.
+Require Import bedrock2.bottom_up_simpl.
 Require Import bedrock2.FE310CSemantics.
 Require Import bedrock2.Loops.
 Require Import bedrock2.Map.Separation.
@@ -7,6 +8,7 @@ Require Import bedrock2.NotationsCustomEntry.
 Require Import bedrock2.ProgramLogic.
 Require Import bedrock2.Scalars.
 Require Import bedrock2.Semantics.
+Require Import bedrock2.SepAutoArray.
 Require Import bedrock2.Syntax.
 Require Import bedrock2.WeakestPrecondition.
 Require Import bedrock2.WeakestPreconditionProperties.
@@ -27,12 +29,7 @@ From Coq Require Import List.
 From Coq Require Import String.
 From Coq Require Import ZArith.
 Require Import Crypto.Arithmetic.PrimeFieldTheorems.
-Require Import Crypto.Bedrock.Field.Interface.Compilation2.
 Require Import Crypto.Bedrock.Field.Synthesis.New.UnsaturatedSolinas.
-Require Import Crypto.Bedrock.Group.AdditionChains.
-Require Import Crypto.Bedrock.Group.ScalarMult.CSwap.
-Require Import Crypto.Bedrock.Group.ScalarMult.LadderStep.
-Require Import Crypto.Bedrock.Group.ScalarMult.MontgomeryLadder.
 Require Import Crypto.Bedrock.End2End.X25519.Field25519.
 Require Import Crypto.Bedrock.Specs.Field.
 Require Import Crypto.Spec.Curve25519.
@@ -51,7 +48,7 @@ Import ProgramLogic.Coercions.
 Import WeakestPrecondition.
 
 Local Existing Instance field_parameters.
-Local Instance frep25519 : Field.FieldRepresentation := field_representation n Field25519.s c.
+Local Existing Instance frep25519.
 Local Existing Instance frep25519_ok.
 
 (* Size of a field element in bytes. This is the same as computing eval in felem_size_bytes, but we want a notation instead of definition. *)
@@ -60,19 +57,19 @@ Local Notation felem_size := 40.
 (* Notations help treat curve points like C structs. To avoid notation clashes, projective coordinates are capitalized. *)
 
 (* Member access notation for projective points: (X, Y, Z, Ta, Tb). *)
-Local Notation "A .X" := (expr.op Syntax.bopname.add A (0)) (in custom bedrock_expr at level 2, left associativity, only parsing).
+Local Notation "A .X" := (A) (in custom bedrock_expr at level 2, left associativity, only parsing).
 Local Notation "A .Y" := (expr.op Syntax.bopname.add A (felem_size)) (in custom bedrock_expr at level 2, left associativity, only parsing).
 Local Notation "A .Z" := (expr.op Syntax.bopname.add A (felem_size + felem_size)) (in custom bedrock_expr at level 2, left associativity, only parsing).
 Local Notation "A .Ta" := (expr.op Syntax.bopname.add A (felem_size + felem_size + felem_size)) (in custom bedrock_expr at level 2, left associativity, only parsing).
 Local Notation "A .Tb" := (expr.op Syntax.bopname.add A (felem_size + felem_size + felem_size + felem_size)) (in custom bedrock_expr at level 2, left associativity, only parsing).
 
 (* Member access notation for precomputed points: (half_ypx, half_ymx, xyd). *)
-Local Notation "A .half_ypx" := (expr.op Syntax.bopname.add A (0)) (in custom bedrock_expr at level 2, left associativity, only parsing).
+Local Notation "A .half_ypx" := (A) (in custom bedrock_expr at level 2, left associativity, only parsing).
 Local Notation "A .half_ymx" := (expr.op Syntax.bopname.add A (felem_size)) (in custom bedrock_expr at level 2, left associativity, only parsing).
 Local Notation "A .xyd" := (expr.op Syntax.bopname.add A (felem_size + felem_size)) (in custom bedrock_expr at level 2, left associativity, only parsing).
 
 (* Member access notation for cached points: (half_YmX, half_YpX, Z, Td). *)
-Local Notation "A .half_YmX" := (expr.op Syntax.bopname.add A (0)) (in custom bedrock_expr at level 2, left associativity, only parsing).
+Local Notation "A .half_YmX" := (A) (in custom bedrock_expr at level 2, left associativity, only parsing).
 Local Notation "A .half_YpX" := (expr.op Syntax.bopname.add A (felem_size)) (in custom bedrock_expr at level 2, left associativity, only parsing).
 Local Notation "A .Z" := (expr.op Syntax.bopname.add A (felem_size + felem_size)) (in custom bedrock_expr at level 2, left associativity, only parsing).
 Local Notation "A .Td" := (expr.op Syntax.bopname.add A (felem_size + felem_size + felem_size)) (in custom bedrock_expr at level 2, left associativity, only parsing).
@@ -177,6 +174,7 @@ Section WithParameters.
 Local Notation "m =* P" := ((P%sep) m) (at level 70, only parsing).
 
 Local Notation FElem := (FElem(FieldRepresentation:=frep25519)).
+Local Notation felem_size_in_bytes := (felem_size_in_bytes(FieldRepresentation:=frep25519)).
 Local Notation bounded_by := (bounded_by(FieldRepresentation:=frep25519)).
 Local Notation word := (Naive.word 32).
 Local Notation felem := (felem(FieldRepresentation:=frep25519)).
@@ -216,7 +214,7 @@ Definition projective_repr P := { p | let '(x,y,z,ta,tb) := p in
                             coordinates P = (feval x, feval y, feval z, feval ta, feval tb) /\
                             bounded_by tight_bounds x /\ bounded_by tight_bounds y /\ bounded_by tight_bounds z /\
                               bounded_by loose_bounds ta /\ bounded_by loose_bounds tb }.
-Local Notation "c 'p5@' p" := (let '(x,y,z,ta,tb) := proj1_sig c in sep (sep (sep (sep (FElem (p .+ 0) x) (FElem (p .+ felem_size) y)) 
+Local Notation "c 'p5@' p" := (let '(x,y,z,ta,tb) := proj1_sig c in sep (sep (sep (sep (FElem (p) x) (FElem (p .+ felem_size) y))
                               (FElem (p .+ (felem_size + felem_size)) z)) (FElem (p .+ (felem_size + felem_size + felem_size)) ta))
                               (FElem (p .+ (felem_size + felem_size + felem_size + felem_size)) tb)) (at level 10, format "c 'p5@' p").
 
@@ -224,13 +222,13 @@ Local Notation "c 'p5@' p" := (let '(x,y,z,ta,tb) := proj1_sig c in sep (sep (se
 Definition precomputed_repr (P : precomputed_point) := { p | let '(half_ymx, half_ypx, xyd) := p in
                             precomputed_coordinates P = (feval half_ymx, feval half_ypx, feval xyd) /\
                             bounded_by loose_bounds half_ymx /\ bounded_by loose_bounds half_ypx /\ bounded_by loose_bounds xyd }.
-Local Notation "c 'p3@' p" := (let '(half_ymx, half_ypx, xyd) := proj1_sig c in sep (sep (FElem (p .+ 0) half_ymx) (FElem (p .+ felem_size) half_ypx))
+Local Notation "c 'p3@' p" := (let '(half_ymx, half_ypx, xyd) := proj1_sig c in sep (sep (FElem (p) half_ymx) (FElem (p .+ felem_size) half_ypx))
                               (FElem (p .+ (felem_size + felem_size)) xyd)) (at level 10, format "c 'p3@' p").
 
 Definition cached_repr (P : cached) := { p | let '(half_ymx, half_ypx,z,td) := p in
                             cached_coordinates P = (feval half_ymx, feval half_ypx, feval z, feval td) /\
                             bounded_by loose_bounds half_ymx /\ bounded_by loose_bounds half_ypx /\bounded_by loose_bounds z /\ bounded_by loose_bounds td }.
-Local Notation "c 'p4@' p" := (let '(half_ymx, half_ypx,z,td) := proj1_sig c in sep (sep (sep (FElem (p .+ 0) half_ymx) (FElem (p .+ felem_size) half_ypx))
+Local Notation "c 'p4@' p" := (let '(half_ymx, half_ypx,z,td) := proj1_sig c in sep (sep (sep (FElem (p) half_ymx) (FElem (p .+ felem_size) half_ypx))
                               (FElem (p .+ (felem_size + felem_size)) z)) (FElem (p .+ (felem_size + felem_size + felem_size)) td)) (at level 10, format "c 'p4@' p").
 
 Instance spec_of_fe25519_half : spec_of "fe25519_half" :=
@@ -248,25 +246,24 @@ Instance spec_of_fe25519_half : spec_of "fe25519_half" :=
         feval result = F.div (feval input) (F.add F.one F.one) /\
         m' =* (FElem result_location result)  * R}.
 
-(* TODO: Use anybytes or similar for output pointer preconditions once the field operation preconditions are suffiently weakened. *)
-
 Global Instance spec_of_add_precomputed : spec_of "add_precomputed" :=
   fnspec! "add_precomputed"
-    (p_out p_a p_b: word) / (a any: point) (b: precomputed_point) (a_repr: projective_repr a) (b_repr: precomputed_repr b) (anything: projective_repr any) (R: _ -> Prop), {
+    (p_out p_a p_b: word) / (a: point) (b: precomputed_point) (a_repr: projective_repr a) (b_repr: precomputed_repr b) (out : list byte) (R: _ -> Prop), {
       requires t m :=
-        m =* anything p5@ p_out * a_repr p5@ p_a * b_repr p3@ p_b * R; 
+        m =* out $@ p_out * a_repr p5@ p_a * b_repr p3@ p_b * R/\
+        Datatypes.length out = Z.to_nat (5 * felem_size);
       ensures t' m' :=
         t = t' /\
         exists a_plus_b : projective_repr (m1add_precomputed_coordinates a b),
           m' =* a_plus_b p5@ p_out * a_repr p5@ p_a * b_repr p3@ p_b * R
     }.
-
 Global Instance spec_of_double : spec_of "double" :=
   fnspec! "double"
     (p_out p_a: word) /
-    (a any: point) (a_repr: projective_repr a) (anything: projective_repr any) (R: _ -> Prop), {
+    (a: point) (a_repr: projective_repr a) (out : list byte) (R: _ -> Prop), {
       requires t m :=
-        m =* anything p5@ p_out * a_repr p5@ p_a * R;
+        m =* out $@ p_out * a_repr p5@ p_a * R /\
+        Datatypes.length out = Z.to_nat (5 * felem_size);
       ensures t' m' := 
         t = t' /\
         exists a_double: projective_repr (m1double a),
@@ -276,9 +273,10 @@ Global Instance spec_of_double : spec_of "double" :=
 Global Instance spec_of_to_cached: spec_of "to_cached" :=
   fnspec! "to_cached"
     (p_out p_a p_d: word) /
-    (a: point) (any: cached) (a_repr: projective_repr a) (anything: cached_repr any) (d1: felem) (R: _ -> Prop), {
+    (a: point) (a_repr: projective_repr a) (d1: felem) (out : list byte) (R: _ -> Prop), {
       requires t m :=
-        m =* anything p4@ p_out * a_repr p5@ p_a * FElem p_d d1 * R /\
+        m =* out $@ p_out * a_repr p5@ p_a * FElem p_d d1 * R /\
+        Datatypes.length out = Z.to_nat (4 * felem_size) /\
         d = feval d1 /\
         bounded_by tight_bounds d1;
       ensures t' m' :=
@@ -290,14 +288,15 @@ Global Instance spec_of_to_cached: spec_of "to_cached" :=
 Global Instance spec_of_readd : spec_of "readd" :=
   fnspec! "readd"
     (p_out p_a p_c: word) /
-    (a any: point) (c: cached) (a_repr: projective_repr a) (anything: projective_repr any) (c_repr: cached_repr c) (R : _ -> Prop), {
+    (a: point) (c: cached) (a_repr: projective_repr a) (c_repr: cached_repr c) (out : list byte) (R : _ -> Prop), {
       requires t m :=
-        m =* anything p5@ p_out * a_repr p5@ p_a * c_repr p4@ p_c * R;
+        m =* out $@ p_out * a_repr p5@ p_a * c_repr p4@ p_c * R /\
+        Datatypes.length out = Z.to_nat (5 * felem_size);
       ensures t' m' :=
         t = t' /\
         exists a_plus_c: projective_repr (m1_readd a c),
           m' =* a_plus_c p5@ p_out * a_repr p5@ p_a * c_repr p4@ p_c * R
-    }.
+  }.
 
 Local Instance spec_of_fe25519_square : spec_of "fe25519_square" := Field.spec_of_UnOp un_square.
 Local Instance spec_of_fe25519_mul : spec_of "fe25519_mul" := Field.spec_of_BinOp bin_mul.
@@ -341,40 +340,28 @@ Local Ltac solve_bounds :=
   | H: bounded_by _ ?x |- bounded_by _ ?x => cbv_bounds H
   end.
 
+ Ltac skipn_firstn_length :=
+    change felem_size_in_bytes with 40 in *; listZnWords.
+
+Ltac split_stack_at_n_in stack p n H := rewrite <- (firstn_skipn n stack) in H;
+  rewrite (map.of_list_word_at_app_n _ _ _ n) in H; try skipn_firstn_length;
+  let D := fresh in unshelve(epose (sep_eq_putmany _ _ (map.adjacent_arrays_disjoint_n p (firstn n stack) (skipn n stack) n _ _)) as D); try skipn_firstn_length;
+  seprewrite_in D H; rewrite ?skipn_skipn in H; bottom_up_simpl_in_hyp H; clear D.
+
 Local Ltac solve_mem :=
-  repeat match goal with
-  | |- exists _ : _ -> Prop, _%sep _ => eexists
-  | |- _%sep _ => ecancel_assumption
-  | |- context[?a + ?b] => match isZcst a with 
-        | false => fail
-        | true => match (isZcst b) with
-            | false => fail
-            | true => let c := eval cbv in (a + b) in change (a + b) with c (* Simplify addition of constants. *)
-          end
-      end
-  | H: ?P%sep _ |- _ => match P with context[?a + ?b] => match isZcst a with 
-          | false => fail
-          | true => match (isZcst b) with
-              | false => fail
-              | true => let c := eval cbv in (a + b) in change (a + b) with c in H
-          end
-        end 
-      end
+  try match goal with  | |- exists _ : _ -> Prop, _%sep _ => eexists end;
+  match goal with  | H : _ %sep ?m |- _ %sep ?m => bottom_up_simpl_in_goal_nop_ok end;
+  match goal with
+  | |- _%sep _ => ecancel_assumption_impl
+  | H: ?P%sep ?m |- ?G%sep ?m =>  (* Solve Placeholder goals when a fixed size list is given *)
+    match P with context[map.of_list_word_at ?p ?stack] =>
+    match G with context[Placeholder ?p _] =>
+      solve [ cbv [Placeholder]; extract_ex1_and_emp_in_goal; bottom_up_simpl_in_goal_nop_ok; split; [ecancel_assumption | skipn_firstn_length] ]
+    end end
   end.
 
-Local Ltac solve_stack :=
-  (* Rewrites the `stack$@a` term in H to use a Bignum instead *)
-  cbv [FElem];
-  match goal with
-  | H: _%sep ?m |- (Bignum.Bignum felem_size_in_words ?a _ * _)%sep ?m =>
-       seprewrite_in (@Bignum.Bignum_of_bytes _ _ _ _ _ _ 10 a) H
-  end;
-  [> transitivity 40%nat; trivial | ];
-  (* proves the memory matches up *)
-  use_sep_assumption; cancel; cancel_seps_at_indices 0%nat 0%nat; cbn; [> trivial | eapply RelationClasses.reflexivity].
-
 Local Ltac single_step :=
-  repeat straightline; straightline_call; ssplit; try solve_mem; try solve_bounds; try solve_stack.
+  repeat straightline; straightline_call; ssplit; try solve_mem; try solve_bounds.
 
 (* Attempts to find anybytes terms in the goal and rewrites the first corresponding stack hypothesis to byte representation.
    straightline only supports deallocation for byte representation at the moment. *)
@@ -391,54 +378,36 @@ Ltac solve_deallocation :=
   end;
   repeat straightline.
 
-(* An example that demonstrates why we need to set Strategy in add_precomputed_ok below *)
-Example demo_strategy : forall x,
-  (@Field.bounded_by field_parameters (Zpos (xO (xO (xO (xO (xO xH))))))
-        BW32 (Naive.word (Zpos (xO (xO (xO (xO (xO xH)))))))
-        (@SortedListWord.map (Zpos (xO (xO (xO (xO (xO xH))))))
-           (Naive.word (Zpos (xO (xO (xO (xO (xO xH))))))) Naive.word32_ok
-           byte) frep25519
-        (@loose_bounds field_parameters (Zpos (xO (xO (xO (xO (xO xH))))))
-           BW32 (Naive.word (Zpos (xO (xO (xO (xO (xO xH)))))))
-           (@SortedListWord.map (Zpos (xO (xO (xO (xO (xO xH))))))
-              (Naive.word (Zpos (xO (xO (xO (xO (xO xH))))))) Naive.word32_ok
-              byte) frep25519) x =
-          @Field.bounded_by field_parameters (Zpos (xO (xO (xO (xO (xO xH))))))
-        BW32 (Naive.word (Zpos (xO (xO (xO (xO (xO xH)))))))
-        (@SortedListWord.map (Zpos (xO (xO (xO (xO (xO xH))))))
-           (Naive.word (Zpos (xO (xO (xO (xO (xO xH))))))) Naive.word32_ok
-           byte) frep25519
-        (@bin_outbounds (Zpos (xO (xO (xO (xO (xO xH)))))) BW32
-           (Naive.word (Zpos (xO (xO (xO (xO (xO xH)))))))
-           (@SortedListWord.map (Zpos (xO (xO (xO (xO (xO xH))))))
-              (Naive.word (Zpos (xO (xO (xO (xO (xO xH))))))) Naive.word32_ok
-              byte) field_parameters frep25519 (@add field_parameters)
-           (@bin_add (Zpos (xO (xO (xO (xO (xO xH)))))) BW32
-              (Naive.word (Zpos (xO (xO (xO (xO (xO xH)))))))
-              (@SortedListWord.map (Zpos (xO (xO (xO (xO (xO xH))))))
-                 (Naive.word (Zpos (xO (xO (xO (xO (xO xH)))))))
-                 Naive.word32_ok byte) field_parameters frep25519)) x).
-Proof.
-  (* reflexivity. *) (* Does not complete within 1 minute. *)
-  (* Now set Strategy precedence... *)
-  Strategy -1000 [bin_outbounds bin_add].
-  reflexivity. (* ...and completes immediately *)
-Qed.
+Ltac split_output_stack stack_var ptr_var num_points :=
+  match goal with
+  | H : context[stack_var $@ ptr_var] |- _ =>
+    split_stack_at_n_in stack_var ptr_var 40%nat H;
+    split_stack_at_n_in (skipn 40 stack_var) (ptr_var.+40) 40%nat H;
+    split_stack_at_n_in (skipn 80 stack_var) (ptr_var.+80) 40%nat H;
+    match num_points with
+    | 4 => idtac
+    | 5 =>
+      split_stack_at_n_in (skipn 120 stack_var) (ptr_var.+120) 40%nat H
+    end
+  end.
 
 Lemma to_cached_ok: program_logic_goal_for_function! to_cached.
 Proof.
   (* Without this, resolution of cbv stalls out Qed. *)
   Strategy -1000 [un_xbounds bin_xbounds bin_ybounds un_square bin_mul bin_add bin_carry_add bin_sub bin_carry_sub un_outbounds bin_outbounds].
 
-  straightline.
+  repeat straightline.
   destruct_points.
-
-  repeat single_step.
+  split_output_stack out p_out 4.
   repeat straightline.
 
+  repeat single_step.
+
+  repeat straightline.
   lazy delta [cached_repr].
   unshelve eexists.
-  eexists (_, _, _, _). 2: solve_mem.
+  eexists (_, _, _, _).
+  2: solve_mem.
   lazy match zeta beta delta [bin_model bin_mul bin_add bin_carry_add bin_sub cached_coordinates coordinates proj1_sig m1_prep] in *.
   ssplit; try solve_bounds.
   congruence.
@@ -449,10 +418,13 @@ Proof.
   (* Without this, resolution of cbv stalls out Qed. *)
   Strategy -1000 [un_xbounds bin_xbounds bin_ybounds un_square bin_mul bin_add bin_carry_add bin_sub un_outbounds bin_outbounds].
 
-  repeat straightline.
+  do 4 straightline.
   destruct_points.
+  split_output_stack out p_out 5.
+  repeat straightline.
 
-  repeat single_step.
+  Time repeat single_step. (* Avoid performance regressions: Keep this around 90s*)
+
   repeat straightline.
   solve_deallocation.
 
@@ -469,8 +441,10 @@ Proof.
   (* Without this, resolution of cbv stalls out Qed. *)
   Strategy -1000 [un_xbounds bin_xbounds bin_ybounds un_square bin_mul bin_add bin_carry_add bin_sub bin_carry_sub un_outbounds bin_outbounds].
 
-  straightline.
+  do 3 straightline.
   destruct_points.
+  split_output_stack out p_out 5.
+  repeat straightline.
 
   repeat single_step.
 
@@ -491,15 +465,18 @@ Proof.
   (* Without this, resolution of cbv stalls out Qed. *)
   Strategy -1000 [un_xbounds bin_xbounds bin_ybounds un_square bin_mul bin_add bin_carry_add bin_sub bin_carry_sub un_outbounds bin_outbounds].
 
-  straightline.
+  do 4 straightline.
   destruct_points.
+  split_output_stack out p_out 5.
+  repeat straightline.
 
-  repeat single_step. repeat straightline.
+  repeat single_step.
 
+  repeat straightline.
   solve_deallocation.
-
   unshelve eexists.
-  eexists (_, _, _, _, _). 2: solve_mem.
+  eexists (_, _, _, _, _).
+  2: solve_mem.
   lazy match beta zeta delta [m1_readd coordinates proj1_sig bin_model bin_mul bin_add bin_carry_add bin_sub] in *.
   ssplit; try solve_bounds.
   Prod.inversion_prod. congruence.
