src/Bedrock/End2End/X25519/GarageDoorTop.v
@@ -9,7 +9,6 @@ Require Import compiler.Symbols.
 Require Import compiler.MMIO.
 Require Import coqutil.Word.Bitwidth32.
 Require Import Crypto.Arithmetic.PrimeFieldTheorems.
-Require Import Crypto.Bedrock.Field.Interface.Compilation2.
 Require Import Crypto.Bedrock.Field.Synthesis.New.UnsaturatedSolinas.
 Require Import Crypto.Bedrock.Group.AdditionChains.
 Require Import Crypto.Bedrock.Group.ScalarMult.LadderStep.
