src/Bedrock/End2End/X25519/MontgomeryLadderRISCV.v
@@ -12,7 +12,6 @@ Require Import Crypto.Arithmetic.PrimeFieldTheorems.
 Require Import Crypto.Bedrock.End2End.X25519.Field25519.
 Require Import Crypto.Bedrock.Field.Synthesis.New.UnsaturatedSolinas.
 Require Import Crypto.Bedrock.Specs.Field.
-Require Import Crypto.Bedrock.Field.Interface.Compilation2.
 Require Import Crypto.Bedrock.Group.ScalarMult.MontgomeryLadder.
 Require Import Crypto.Bedrock.End2End.X25519.MontgomeryLadder.
 
