src/Bedrock/Secp256k1/Field256k1.v
@@ -30,6 +30,8 @@ Section Field.
          M ((a + F.of_Z _ 2) / F.of_Z _ 4)%F prefix).
   Defined.
 
+  #[export] Instance frep256k1 : Field.FieldRepresentation := field_representation m.
+
   Definition to_mont_string := (prefix ++ "to_mont")%string.
   Definition from_mont_string := (prefix ++ "from_mont")%string.
 
@@ -78,16 +80,34 @@ Section Field.
         eapply Func.valid_func_bool_iff;
         abstract vm_cast_no_check (eq_refl true)
     | |- (_ = _)%Z => vm_compute; reflexivity
+    | |- (felem_size_in_bytes <= 2 ^ _)%Z => apply felem_size_ok
     end.
 
   Local Notation functions_contain functions f :=
     (Interface.map.get functions (fst f) = Some (snd f)).
 
+  #[export] Instance frep256k1_raw : FieldRepresentation := field_representation_raw m.
+  #[export] Instance frep256k1_raw_ok : FieldRepresentation_ok (field_representation:=frep256k1_raw).
+  Proof.
+    apply Crypto.Bedrock.Field.Synthesis.New.Signature.field_representation_ok.
+    auto.
+    let sz := eval lazy in felem_size_in_bytes in change felem_size_in_bytes with sz.
+    Lia.lia.
+  Qed.
+
+  #[export] Instance frep256k1_ok : FieldRepresentation_ok(field_representation:=frep256k1).
+  Proof.
+    apply Crypto.Bedrock.Field.Synthesis.New.Signature.field_representation_ok.
+    auto.
+    let sz := eval lazy in felem_size_in_bytes in change felem_size_in_bytes with sz.
+    Lia.lia.
+  Qed.
+
   Derive secp256k1_felem_copy
          SuchThat (forall functions,
                       functions_contain functions secp256k1_felem_copy ->
                       spec_of_felem_copy
-                        (field_representation:=field_representation_raw m)
+                        (field_representation:=frep256k1_raw)
                         functions)
          As secp256k1_felem_copy_correct.
   Proof. Time derive_bedrock2_func felem_copy_op. Qed.
@@ -96,7 +116,7 @@ Section Field.
          SuchThat (forall functions,
                       functions_contain functions secp256k1_from_bytes ->
                       spec_of_from_bytes
-                        (field_representation:=field_representation_raw m)
+                        (field_representation:=frep256k1_raw)
                         functions)
          As secp256k1_from_bytes_correct.
   Proof. Time derive_bedrock2_func from_bytes_op. Qed.
@@ -105,7 +125,7 @@ Section Field.
          SuchThat (forall functions,
                       functions_contain functions secp256k1_to_bytes ->
                       spec_of_to_bytes
-                        (field_representation:=field_representation_raw m)
+                        (field_representation:=frep256k1_raw)
                         functions)
          As secp256k1_to_bytes_correct.
   Proof. Time derive_bedrock2_func to_bytes_op. Qed.
@@ -114,7 +134,7 @@ Section Field.
          SuchThat (forall functions,
                       functions_contain functions secp256k1_opp ->
                       spec_of_UnOp un_opp
-                        (field_representation:=field_representation m)
+                        (field_representation:=frep256k1)
                         functions)
          As secp256k1_opp_correct.
   Proof. Time derive_bedrock2_func opp_op. Qed.
@@ -123,7 +143,7 @@ Section Field.
          SuchThat (forall functions,
                       functions_contain functions secp256k1_mul ->
                       spec_of_BinOp bin_mul
-                        (field_representation:=field_representation m)
+                        (field_representation:=frep256k1)
                         functions)
          As secp256k1_mul_correct.
   Proof. Time derive_bedrock2_func mul_op. Qed.
@@ -132,7 +152,7 @@ Section Field.
          SuchThat (forall functions,
                       functions_contain functions secp256k1_square ->
                       spec_of_UnOp un_square
-                        (field_representation:=field_representation m)
+                        (field_representation:=frep256k1)
                         functions)
          As secp256k1_square_correct.
   Proof. Time derive_bedrock2_func square_op. Qed.
@@ -141,7 +161,7 @@ Section Field.
          SuchThat (forall functions,
                       functions_contain functions secp256k1_add ->
                       spec_of_BinOp bin_add
-                        (field_representation:=field_representation m)
+                        (field_representation:=frep256k1)
                         functions)
          As secp256k1_add_correct.
   Proof. Time derive_bedrock2_func add_op. Qed.
@@ -150,7 +170,7 @@ Section Field.
          SuchThat (forall functions,
                       functions_contain functions secp256k1_sub ->
                       spec_of_BinOp bin_sub
-                        (field_representation:=field_representation m)
+                        (field_representation:=frep256k1)
                         functions)
          As secp256k1_sub_correct.
   Proof. Time derive_bedrock2_func sub_op. Qed.
@@ -159,7 +179,7 @@ Section Field.
            SuchThat (forall functions,
                       functions_contain functions secp256k1_select_znz ->
                       spec_of_selectznz
-                        (field_representation:=field_representation m)
+                        (field_representation:=frep256k1)
                         functions)
          As secp256k1_select_znz_correct.
   Proof. Time derive_bedrock2_func select_znz_op. Qed.
@@ -168,7 +188,7 @@ Section Field.
          SuchThat (forall functions,
                       functions_contain functions secp256k1_from_mont ->
                       spec_of_UnOp un_from_mont
-                        (field_representation:=field_representation m)
+                        (field_representation:=frep256k1)
                         functions)
          As secp256k1_from_mont_correct.
   Proof. Time derive_bedrock2_func from_mont_op. Unshelve. 1,2: auto. Qed.
@@ -177,16 +197,10 @@ Section Field.
          SuchThat (forall functions,
                       functions_contain functions secp256k1_to_mont ->
                       spec_of_UnOp un_to_mont
-                        (field_representation:=field_representation m)
+                        (field_representation:=frep256k1)
                         functions)
          As secp256k1_to_mont_correct.
   Proof. Time derive_bedrock2_func to_mont_op. Unshelve. 1,2: auto. Qed.
-
-  #[export] Instance frep256k1_ok : FieldRepresentation_ok(field_representation:=field_representation m).
-  Proof.
-    apply Crypto.Bedrock.Field.Synthesis.New.Signature.field_representation_ok.
-    auto.
-  Qed.
 End Field.
 
 (* Require Import bedrock2.Syntax. *)
